code/experimental/curve25519/Hacl.Spec.Curve25519.AddAndDouble.fst
@@ -30,3 +30,44 @@ val lemma_double:
   q:proj_point -> nq:proj_point -> nqp1:proj_point ->
   Lemma (double nq == fst (add_and_double q nq nqp1))
 let lemma_double q nq nqp1 = ()
+
+// let cswap2 (sw:uint8) (nq:proj_point) (nqp1:proj_point) =
+//   let open Lib.RawIntTypes in
+//   if uint_to_nat sw = 1 then (nqp1, nq) else (nq, nqp1)
+
+let ladder_step1 (k:scalar) (q:proj_point) (i:nat{i < 251}) (nq, nqp1, swap) =
+  let bit = ith_bit k (253-i) in
+  let sw = swap ^. bit in
+  let nq, nqp1 = cswap2 sw nq nqp1 in
+  let nq, nqp1 = add_and_double q nq nqp1 in
+  (nq, nqp1, bit)
+
+let montgomery_ladder1_0 (k:scalar) (q:proj_point) (nq:proj_point) (nqp1:proj_point) =
+  // bit 255 is 0 and bit 254 is 1
+  let nq,nqp1 = cswap2 (u64 1) nq nqp1 in
+  let nq,nqp1 = add_and_double q nq nqp1 in
+  let swap = u64 1 in
+  let nq,nqp1,swap = Lib.LoopCombinators.repeati 251 (ladder_step1 k q) (nq, nqp1, swap) in
+  let nq,nqp1 = cswap2 swap nq nqp1 in
+  nq
+
+let montgomery_ladder1_1 (nq:proj_point) =
+  let nq = double nq in
+  let nq = double nq in
+  let nq = double nq in
+  nq
+
+let montgomery_ladder1_2 (init:elem) =
+  let q = (init, one) in
+  let nq = (one, zero) in
+  let nqp1 = (init, one) in
+  q, nq, nqp1
+
+let montgomery_ladder1 (init:elem) (k:scalar) : Tot proj_point =
+  let q, nq, nqp1 = montgomery_ladder1_2 init in
+  let nq = montgomery_ladder1_0 k q nq nqp1 in
+  montgomery_ladder1_1 nq
+
+val lemma_montgomery_ladder: init:elem -> k:scalar ->
+  Lemma (montgomery_ladder1 init k == montgomery_ladder init k)
+let lemma_montgomery_ladder init k = admit()
